Modifying types to make different easier types easier to load/store in memory

src/Dafny/types.dfy
@@ -12,19 +12,235 @@ newtype{:nativeType "ulong"} ulong = i:int | 0 <= i < 0x1_0000_0000_0000_0000
 // Subset types
 /////////////////
 
+// The integer types as normally defined
 type uint8   = i:int | 0 <= i < 0x100
 type uint16  = i:int | 0 <= i < 0x10000
 type uint32  = i:int | 0 <= i < 0x1_0000_0000
 type uint64  = i:int | 0 <= i < 0x1_0000_0000_0000_0000
 type uint128 = i:int | 0 <= i < 0x1_00000000_00000000_00000000_00000000
-
 type int8    = i:int | -0x80 <= i < 0x80
 type int16   = i:int | -0x8000 <= i < 0x8000
 type int32   = i:int | -0x8000_0000 <= i < 0x8000_0000
 type int64   = i:int | -0x8000_0000_0000_0000 <= i < 0x8000_0000_0000_0000
 type int128  = i:int | -0x8000_0000_0000_0000_0000_0000_0000_0000 <= i < 0x8000_0000_0000_0000_0000_0000_0000_0000
 
-datatype ptr = ptr(bid:nat, offset:nat)
+// A pointer is a block/index, not an absolute value, based on our specification
+// Each Data holds a piece of information that can be loaded/stored from/to memory
+datatype Data = Bytes(bytes:seq<uint8>) |
+                Ptr(block:nat, offset:nat) |
+                Int(val:int, size:nat, signed:bool)
+
+// For aiding in converting between the size of a number in bytes and its bounds
+function Pow256(n:nat) : (ret:nat)
+    ensures ret > 0
+    decreases n
+{
+    if n == 0 then 1
+    else 0x100 * Pow256(n-1)
+}
+
+// In order to be valid, integer types need to be within the bounds of their size
+// Also, cannot have bytes that are empty
+predicate {:opaque} ValidData(data:Data) {
+    match data
+        case Bytes(bytes) => |bytes| > 0
+        case Ptr(block, offset) => true
+        case Int(val, size, signed) =>
+            var bound := Pow256(size) as int;
+            if size == 0 then false
+            else if signed then (-bound/2 <= val < bound/2)
+            else (0 <= val < bound)
+}
+
+// Getters for the common integer types
+function UInt8(val:uint8) : (data:Data)
+    ensures ValidData(data)
+{
+    reveal_ValidData();
+    Int(val, 1, false)
+}
+
+function UInt16(val:uint16) : (data:Data)
+    ensures ValidData(data)
+{
+    reveal_ValidData();
+    Int(val, 2, false)
+}
+
+function UInt32(val:uint32) : (data:Data)
+    ensures ValidData(data)
+{
+    reveal_ValidData();
+    Int(val, 4, false)
+}
+
+function UInt64(val:uint64) : (data:Data)
+    ensures ValidData(data)
+{
+    reveal_ValidData();
+    Int(val, 8, false)
+}
+
+function UInt128(val:uint128) : (data:Data)
+    ensures ValidData(data)
+{
+    reveal_ValidData();
+    Int(val, 16, false)
+}
+
+function Int8(val:int8) : (data:Data)
+    ensures ValidData(data)
+{
+    reveal_ValidData();
+    Int(val, 1, true)
+}
+
+function Int16(val:int16) : (data:Data)
+    ensures ValidData(data)
+{
+    reveal_ValidData();
+    Int(val, 2, true)
+}
+
+function Int32(val:int32) : (data:Data)
+    ensures ValidData(data)
+{
+    reveal_ValidData();
+    Int(val, 4, true)
+}
+
+function Int64(val:int64) : (data:Data)
+    ensures ValidData(data)
+{
+    reveal_ValidData();
+    Int(val, 8, true)
+}
+
+function Int128(val:int128) : (data:Data)
+    ensures ValidData(data)
+{
+    reveal_ValidData();
+    Int(val, 16, true)
+}
+
+// Converts a signed integer to its unsigned representation in two's complement
+function {:opaque} ToTwosComp(data:Data) : (out:Data)
+    requires data.Int? && data.signed && ValidData(data)
+    ensures out.Int? && !out.signed && ValidData(out)
+    ensures out.size == data.size
+{
+    reveal_ValidData();
+    var newval := (if data.val >= 0 then data.val else data.val + Pow256(data.size));
+    Int(newval, data.size, false)
+}
+
+// Converts an unsigned two's complement back to its signed integer counterpart
+function {:opaque} FromTwosComp(data:Data) : (out:Data)
+    requires data.Int? && !data.signed && ValidData(data)
+    ensures out.Int? && out.signed && ValidData(out)
+    ensures out.size == data.size
+{
+    reveal_ValidData();
+    var bound := Pow256(data.size) as int;
+    var newval := (if data.val < bound/2 then data.val else data.val - bound);
+    Int(newval, data.size, true)
+}
+
+// // Makes sure that sending numbers through two's complement and back doesn't change them
+lemma {:opaque} TwosCompIdentity(data:Data)
+    requires data.Int? && data.signed && ValidData(data)
+    ensures FromTwosComp(ToTwosComp(data)) == data
+{
+    reveal_ToTwosComp();
+    reveal_FromTwosComp();
+}
+
+// Transforms data that is in some arbitrary form into byte form
+function ToBytes(data:Data) : (bytes:seq<uint8>)
+    requires !data.Ptr?
+    requires ValidData(data)
+    ensures data.Int? ==> |bytes| == data.size
+{
+    reveal_ValidData();
+    if data.Bytes? then data.bytes
+    else
+        var val := if data.signed then ToTwosComp(data).val else data.val;
+        UIntToBytes(val, data.size)
+}
+
+// Recursive helper function for ToBytes() for handling the integer case
+function UIntToBytes(val:nat, size:nat) : (bytes:seq<uint8>)
+    requires val < Pow256(size)
+    ensures |bytes| == size
+    decreases size
+{
+    if size == 0 then []
+    else [val % 0x100] + UIntToBytes(val / 0x100, size - 1)
+}
+
+// Going the other way, we transform data that is in byte form back into some
+// other format
+function FromBytes(bytes:seq<uint8>, form:Data) : (data:Data)
+    requires |bytes| > 0
+    requires !form.Ptr?
+    requires form.Int? ==> form.size == |bytes|
+    ensures form.Bytes? ==> data.Bytes?
+    ensures form.Int? ==> data.Int?
+    ensures form.Int? ==> data.size == form.size
+    ensures form.Int? ==> data.signed == form.signed
+    ensures ValidData(data)
+{
+    reveal_ValidData();
+    if form.Bytes? then Bytes(bytes)
+    else
+        var val := UIntFromBytes(bytes);
+        var udata := Int(val, form.size, false);
+        if form.signed then FromTwosComp(udata)
+        else udata
+}
+
+// Recursive helper function for FromBytes() for handling the integer case
+function UIntFromBytes(bytes:seq<uint8>) : (val:nat)
+    ensures val < Pow256(|bytes|)
+    decreases bytes
+{
+    if |bytes| == 0 then 0
+    else bytes[0] + (0x100 * UIntFromBytes(bytes[1..]))
+}
+
+// First, let's just make sure that the uint conversions preserve information
+lemma {:opaque} {:induction val, size} UIntBytesIdentity(val:nat, size:nat)
+    requires val < Pow256(size)
+    ensures UIntFromBytes(UIntToBytes(val, size)) == val
+{
+}
+
+// Finally, need to verify that converting data to bytes and back again doesn't change
+// it whatsoever
+// lemma {:opaque} ToBytesIdentity(data:Data)
+//     requires !data.Ptr?
+//     requires ValidData(data)
+//     ensures FromBytes(ToBytes(data), data) == data
+// {
+//     if (data.Bytes?) {
+//         assert FromBytes(ToBytes(data), data) == data;
+//     } else {
+//         assert data.Int?;
+//         if (data.signed) {
+//             if (data.size == 1) {
+//                 assert FromBytes(ToBytes(data), data) == data;
+//             } else {
+//                 assert FromBytes(ToBytes(data), data) == data;
+//             }
+//         } else {
+//             if (data.size == 1) {
+//                 assert FromBytes(ToBytes(data), data) == data;
+//             } else {
+//                 assert FromBytes(ToBytes(data), data) == data;
+//             }
+//         }
+//     }
+// }
 
 datatype Value = Val8(v8:uint8) | Val16(v16:uint16) | Val32(v32:uint32) | Val64(v64:uint64) | Val128(v128:uint128)
 
